src/proof/yjs_core.v
@@ -16,8 +16,10 @@
       ArrSet, YjsArrInvariant             yjs.algorithm.invariant_yjsarray
       IsItemValid                         yjs.algorithm.invariant_basic
       YjsArrInvariant_integrateSafe       yjs.algorithm.insert_loop
+      setfii_loop, setintegrate, Couple,  yjs.algorithm.insert_set
+        setintegrate_eq_integrate, ...
 *)
 From yjs.crdt Require Export client_id.
 From yjs Require Export item item_set util.
 From yjs.order Require Export item_order item_set_invariant.
-From yjs.algorithm Require Export basic insert_basic invariant_basic invariant_yjsarray insert_loop.
+From yjs.algorithm Require Export basic insert_basic invariant_basic invariant_yjsarray insert_loop insert_set.
